# Exercise 1.13

Let $T(n)$ be the claim that $Fib(n) = (\phi^n - \psi^n) / \sqrt{5}$, where $\phi = (1 + \sqrt{5}) / 2$ and $\psi = (1 - \sqrt{5}) / 2$.

$T(0)$ is true since $(\phi^0 - \psi^0) / \sqrt{5} = 0 = Fib(0)$.

$T(1)$ is true since $(\phi^1 - \psi^1) / \sqrt{5} = (1 + \sqrt{5} - 1 + \sqrt{5}) / (2 \sqrt{5}) = 1 = Fib(1)$.

Before moving on to the general case, let's establish a few properties of $\phi$ and $\psi$.

Firstly, $\phi\psi = (1 + \sqrt{5})(1 - \sqrt{5})/4 = (1 - 5) / 4 = -1 \Rightarrow -\phi\psi = 1 \Rightarrow \phi^2\psi^2 = 1$.

Secondly, $\phi + \psi = (1 + \sqrt{5} + 1 - \sqrt{5}) / 2 = 1 \Leftrightarrow \phi = 1 - \psi \Leftrightarrow \psi = 1 - \phi$.

Now assume that $T(n-2)$ and $T(n-1)$ are true for some $n \geq 2$.

Then,
$$
\begin{aligned}
    Fib(n) &= Fib(n-1) + Fib(n-2) \\
    &= (\phi^{n-1} - \psi^{n-1}) / \sqrt{5} + (\phi^{n-2} - \psi^{n-2}) / \sqrt{5} \\
    &= (-\phi\psi\phi^{n-1} + \phi\psi\psi^{n-1}) / \sqrt{5} + (\phi^2\psi^2\phi^{n-2} - \phi^2\psi^2\psi^{n-2}) / \sqrt{5} \\
    &= (-\psi\phi^{n} + \phi\psi^{n}) / \sqrt{5} + (\phi^{n}\psi^2 - \phi^2\psi^{n}) / \sqrt{5} \\
    &= \frac{\phi^n(\psi^2 - \psi) - \psi^n(\phi^2-\phi)}{\sqrt{5}} \\
    &= \frac{\phi^n\psi(\psi - 1) - \psi^n\phi(\phi-1)}{\sqrt{5}} \\
    &= \frac{\phi^n\psi(-\phi) - \psi^n\phi(-\psi)}{\sqrt{5}} \\
    &= \frac{\phi^n - \psi^n}{\sqrt{5}},
\end{aligned}
$$
that is, $T(n)$ is true. Thus, by induction, $T(n)$ is true for all $n \geq 0$.

We know that Fibonacci numbers are integers. This implies that $(\phi^n - \psi^n)\sqrt{5}$ must be an integer for all $n \geq 0$ as we just established that it's equal to $Fib(n)$. The absolute value of $\psi^n / \sqrt{5}$ is less than 0.5 for each $n$ since this applies for $n=0$ and the absolute value is strictly decreasing with respect to $n$. As the absolute value of $\psi^n / \sqrt{5}$ is the distance between $Fib(n)$ and $\phi^n / \sqrt{5}$, and this distance is always less than 0.5, $Fib(n)$ is the closest integer to $\phi^n / \sqrt{5}$.
